\begin{Lemma}{taylor-y}
The Taylor expansion of $y_1$ with respect to $h$ is
  \begin{gather}
    \label{eq:taylor-y:1}
    \begin{split}
      &(y_1)_n = (u_0)_n
      \\& + h \sum_{j=1}^s b_i f_n
      \\& + \frac{h^2}2 \sum_{\lambda} \left[2\sum_{i} b_i c_i
        \partial_{\lambda} f_n f_\lambda\right]
      \\& + \frac{h^3}6 \sum_{\lambda,\mu} \left[
        3\sum_{i} b_i c_i^2
        \partial_{\lambda\mu} f_n f_\lambda f_\mu
        + 6 \sum_{i,j} b_i a_{ij} c_j
        \partial_{\lambda} f_n \partial_\mu f_\lambda f_\mu
      \right]
      \\& + \frac{h^4}{24} \sum_{\lambda,\mu,\nu} \left[
        6 \sum_{i} b_i c_i^3
        \partial_{\lambda\mu\nu} f_n f_\lambda f_\mu f_\nu
      + 3 \sum_{i,j} b_i c_i a_{ij} c_j\partial_{\lambda\mu} f_n \partial_{m}f_\lambda f_\mu f_\nu
        \right.
      \\&\hphantom{+\frac{h^4}{24} \sum_{\lambda,\mu,\nu}} \left.
      + 2 \sum_{i,j} b_i a_{ij} c_j^2\partial_{\lambda}f_n \partial_{\mu\nu} f_\lambda f_\mu f_\nu
      + \sum_{i,j,k} b_i a_{ij} a_{jk} c_k \partial_{\lambda}f_n \partial_{\mu} f_\lambda \partial_{\nu}
      f_\mu f_\nu
      \right].
    \end{split}
  \end{gather}
\end{Lemma}

%%% Local Variables: 
%%% mode: latex
%%% TeX-master: "../notes"
%%% End: 
