\begin{Definition}{lmm}
  \index{Multistep method}
  \index{LMM|see{linear multistep method}}
  A \define{linear multistep method} (LMM) with $\lmms$ steps is a
  method of form
  \begin{gather}
    \label{eq:lmm:4}
    \sum_{r=0}^{\lmms} \alpha_{\lmms-r} y_{k-r}
    = h \sum_{r=0}^{\lmms}\beta_{\lmms-r} f_{k-r},
  \end{gather}
  where $f_k = f(t_k, y_k)$ and $t_k = t_0+hk$. There are
  explicit ($\beta_\lmms = 0$) and implicit ($\beta_\lmms \neq 0$)
  methods.  For these methods, we define the first and second 
	\define{generating polynomials}
  \begin{xalignat}{2}
    \label{eq:lmm:5}
    \rho(x) &= \sum_{r=0}^{\lmms} \alpha_{\lmms-r} x^{s-r}= \sum_{r=0}^{\lmms} \alpha_{r} x^{r}
    &
    \sigma(x) &= \sum_{r=0}^{\lmms} \beta_{r} x^{r}.
  \end{xalignat}
\end{Definition}

%%% Local Variables:
%%% mode: latex
%%% TeX-master: "../notes"
%%% End:
